# Binomial
<font size=5>

$(1+x)^n = 1+ nx + \frac{n(n-1)x^2}{2!} + \frac{n(n-1)(n-2)x^3}{3!}$

</font>
Find the first 4 yerms of the exp of $\frac{1}{1-x}$

$(1+x)^{-1} = 1 + x + \frac{(-1)(-2)(-x)^2}{2!} + \frac{(-1)(-2)(-3)(-x)^3}{3!}$

$1 + x + x^2 + x^3$

Expand $\sqrt{1-2x}$ up to $x^3$ and use the expansion to estimate $\sqrt{5}$ using $x = 0.1$

<font size=5>

$(1-2x)^\frac{1}{2}$

$1-x-\frac{x^2}{2}-\frac{x^3}{2}$

$\left | x  \right | < \frac{1}{2}$


when $x=0.1, 1-2x =0.8$


$\sqrt{0.8} = 1-0.1 - \frac{0.1^2}{2} - \frac{0.1^3}{2} + ...$

$=0.8945$

$\sqrt{0.8} = \sqrt{\frac{8}{10}} = \sqrt{\frac{4}{5}} = \frac{\sqrt{4}}{\sqrt{5}} = \frac{2}{\sqrt{5}}$

$\sqrt{0.8} = \frac{2}{\sqrt{5}}$

$\sqrt{5} = \frac{2}{\sqrt{0.8}} = \frac{2}{0.8945} = 2.236$

--- 

</font>

What if we have $(4+x)^\frac{1}{2}$, not 1?

<font size=5>

$(4+x)\frac{1}{2} = [4(1+\frac{x}{4})]^\frac{1}{2} = 4^\frac{1}{2}(1 + \frac{x}{4})^\frac{1}{2} =2[1+\frac{(\frac{1}{2})(\frac{-1}{2})(\frac{x}{4})^2}{2!} + \frac{(\frac{1}{2})(\frac{-1}{2}) (\frac{-3}{-2})(\frac{x}{4})^3}{3!}]$

$2 + \frac{x}{4} + \frac{x}{4} - \frac{x^2}{64} + \frac{x^3}{517}$

</font>

---

$\sqrt[3]{(8+x)}$ first 4 terms use this to find the value of $\sqrt{8.1}$ to 6dp

<font size=4>

$=(8+x)^\frac{1}{3}$

$=[8(1 + (\frac{x}{8}))]^\frac{1}{3}$

$1 + \frac{1}{3}x + \frac{1}{3}$

$(8+x)^\frac{1}{3} = 2 + \frac{x}{12} - \frac{x^2}{288} + \frac{5x^3}{20736}$

$\sqrt[3]{8+x} = \sqrt[3]{8.1}$

$8+x = 8.1$

$x=0.1$

let $x=0.1$

$\sqrt[3]{8.1} = 2+\frac{0.1}{12} - \frac{0.1^2}{288} + \frac{0.1^3}{20736} = 2.008299$

## homework is 4a) q5,6 4b) q1cd, 2