# even more binomial

Expand up to and including the term in x^2

<font size=5>

$\sqrt{\frac{1+2x}{1-4x}}$

$\frac{(1+2x)^\frac{1}{2}}{(1-4x)^\frac{1}{2}} = (1+2x)^\frac{1}{2}(1-4x)^\frac{-1}{2}$

$(1+x)^n = 1+ nx + \frac{n(n-1)x^2}{2!}$

$(1+2x)^\frac{1}{2} = 1 + x - \frac{x^2}{2} + ..$

$\left | x \right | < \frac{1}{2}$

$(1-4x)^\frac{1}{2} = 1+2x + 6x^2 + ...$

$\left | x \right | < \frac{1}{4}$

$(1 + x - \frac{x^2}{2})(1+2x + 6x^2)$

You only need ^2 since the question asks, so dont bother expanding all

$= 1 + 3x + \frac{15}{2}x^2$

$\left | x \right | < \frac{1}{4}$

always choose the smallest modulus, since it is compatible with both equations

</font>

---

Expand $(4-3x)^\frac{-1}{2}$ up to x^2 and hence evaluate $\frac{1}{\sqrt{3.97}}$ to 4sf

<font size=5>

$4^{\frac{-1}{2}}[(1-\frac{3}{4}x)^{\frac{-1}{2}}]$

$\frac{1}{2}[(1-\frac{3}{4}x)^\frac{-1}{2}]$

$= 1+ \frac{-1}{2}(\frac{3}{4}x) + \frac{\frac{-1}{2}(\frac{-1}{2}-1)(\frac{3}{4}x)^2}{2!}$

$= \frac{1}{2}[1 - \frac{3}{8}x + \frac{27}{128}x^2]$

$= \frac{1}{2} - \frac{3}{16}x + \frac{27}{256}x^2$

$\left | x \right | <\frac{4}{3}$

$\frac{1}{\sqrt{4-3x}} = \frac{1}{\sqrt{3.97}}$

$x = 0.0.1$

$\frac{1}{\sqrt{3.97}} = \frac{1}{2} + \frac{3}{16}(0.01) + \frac{27}{256}(0.01)^2$

$= 0.5019$

</font>

---
# 4B q7

Expand and evaluate to $\sqrt[4]{15.7}$ up to x^2

<font size=5>

$(16-3x)^\frac{1}{4}$

$16^{\frac{1}{4}}[(1-\frac{3}{16}x)^\frac{1}{4}]$

$2[(1-\frac{3}{16}x)^\frac{1}{4}]$

$1 + \frac{1}{4}(\frac{3}{16}x) + \frac{\frac{1}{4}(\frac{1}{4}-1)(\frac{3}{16}x)^2}{2!}$

$= 2[1+ \frac{3}{64}x - \frac{27}{8182}x^2]$

$=2 - \frac{3}{32}x - \frac{27}{4096}x^2$

hence $\sqrt[4]{15.7} =2 - \frac{3}{32}(0.1) - \frac{27}{4096}(0.1)^2$

</font>

Given that the expansion of $(1+ax)^n$ is $1-2x + \frac{7}{3}x^2 + kx^3$ find the value of k

<font size=5>

$(1+ax)^n = 1 + anx + \frac{n(n-1)a^2x^2}{2!} + \frac{n(n-1)(n-2)a^3x^3}{3!}$

therefore $an = -2$
because they are both the coefficients of x

therefore $\frac{n(n-1)a^2}{2} = \frac{7}{3}$

do simulatenous equations 

$a=\frac{-2}{n}$

$\frac{n(n-1)(\frac{-2}{n})^2}{2}  = \frac{7}{3}$

$n(n-1)(\frac{-2}{n^2}) = \frac{14}{3}$

$3n(n-1)(\frac{-2}{n^2}) = 14$






</fomt>

--- 
## HW is Ex4c, 1a, 2a, 3a, 4a